src/Arithmetic/Freeze.v
@@ -116,7 +116,7 @@ Module Freeze.
           (Hp : 0 <= Positional.eval weight n p < 2*modulus)
           (Hplen : length p = n)
           (Hmlen : length m = n)
-      : @freeze n mask m p = partition weight n (Positional.eval weight n p mod modulus).
+      : @freeze n mask m p = Partition.partition weight n (Positional.eval weight n p mod modulus).
     Proof using wprops.
       pose proof (@weight_positive weight wprops n).
       pose proof (fun v => Z.mod_pos_bound v (weight n) ltac:(lia)).
@@ -252,7 +252,7 @@ Section freeze_mod_ops.
     : forall (f : list Z)
              (Hf : length f = n)
              (Hf_small : 0 <= eval weight n f < weight n),
-      to_bytes f = partition bytes_weight bytes_n (Positional.eval weight n f).
+      to_bytes f = Partition.partition bytes_weight bytes_n (Positional.eval weight n f).
   Proof using Hn_nz limbwidth_good.
     clear -Hn_nz limbwidth_good.
     intros; cbv [to_bytes].
@@ -265,7 +265,7 @@ Section freeze_mod_ops.
              (Hf : length f = n)
              (Hf_small : 0 <= eval weight n f < weight n),
       eval bytes_weight bytes_n (to_bytesmod f) = eval weight n f
-      /\ to_bytesmod f = partition bytes_weight bytes_n (Positional.eval weight n f).
+      /\ to_bytesmod f = Partition.partition bytes_weight bytes_n (Positional.eval weight n f).
   Proof using Hn_nz limbwidth_good.
     split; apply eval_to_bytes || apply to_bytes_partitions; assumption.
   Qed.
@@ -275,7 +275,7 @@ Section freeze_mod_ops.
         (Hf : length f = n)
         (Hf_bounded : 0 <= eval weight n f < 2 * m),
       (eval bytes_weight bytes_n (freeze_to_bytesmod f)) = (eval weight n f) mod m
-      /\ freeze_to_bytesmod f = partition bytes_weight bytes_n (Positional.eval weight n f mod m).
+      /\ freeze_to_bytesmod f = Partition.partition bytes_weight bytes_n (Positional.eval weight n f mod m).
   Proof using m_enc_correct Hs limbwidth_good Hn_nz c_small Hm_enc_len m_enc_bounded.
     clear -m_enc_correct Hs limbwidth_good Hn_nz c_small Hm_enc_len m_enc_bounded.
     intros; subst m s.
@@ -299,7 +299,7 @@ Section freeze_mod_ops.
     : forall (f : list Z)
         (Hf : length f = n)
         (Hf_bounded : 0 <= eval weight n f < 2 * m),
-      freeze_to_bytesmod f = partition bytes_weight bytes_n (Positional.eval weight n f mod m).
+      freeze_to_bytesmod f = Partition.partition bytes_weight bytes_n (Positional.eval weight n f mod m).
   Proof using m_enc_correct Hs limbwidth_good Hn_nz c_small Hm_enc_len m_enc_bounded.
     intros; now apply eval_freeze_to_bytesmod_and_partitions.
   Qed.
@@ -320,7 +320,7 @@ Section freeze_mod_ops.
   Lemma from_bytes_partitions
     : forall (f : list Z)
              (Hf_small : 0 <= eval bytes_weight bytes_n f < weight n),
-      from_bytes f = partition weight n (Positional.eval bytes_weight bytes_n f).
+      from_bytes f = Partition.partition weight n (Positional.eval bytes_weight bytes_n f).
   Proof using limbwidth_good.
     clear -limbwidth_good.
     intros; cbv [from_bytes].
@@ -337,7 +337,7 @@ Section freeze_mod_ops.
   Lemma from_bytesmod_partitions
     : forall (f : list Z)
              (Hf_small : 0 <= eval bytes_weight bytes_n f < weight n),
-      from_bytesmod f = partition weight n (Positional.eval bytes_weight bytes_n f).
+      from_bytesmod f = Partition.partition weight n (Positional.eval bytes_weight bytes_n f).
   Proof using limbwidth_good. apply from_bytes_partitions. Qed.
 
   Lemma eval_from_bytesmod_and_partitions
@@ -345,7 +345,7 @@ Section freeze_mod_ops.
              (Hf : length f = bytes_n)
              (Hf_small : 0 <= eval bytes_weight bytes_n f < weight n),
       eval weight n (from_bytesmod f) = eval bytes_weight bytes_n f
-      /\ from_bytesmod f = partition weight n (Positional.eval bytes_weight bytes_n f).
+      /\ from_bytesmod f = Partition.partition weight n (Positional.eval bytes_weight bytes_n f).
   Proof using limbwidth_good Hn_nz.
     now (split; [ apply eval_from_bytesmod | apply from_bytes_partitions ]).
   Qed.
